src/computational_monads/simulation_semantics/default_simulate.lean
@@ -1,0 +1,119 @@
+import computational_monads.simulation_semantics.simulate
+
+namespace oracle_comp
+
+variables {A B C : Type} {spec spec' spec'' : oracle_spec}
+  (so : simulation_oracle spec spec') (so' : simulation_oracle spec spec'')
+  (a : A) (i : spec.ι) (t : spec.domain i)
+  (oa oa' : oracle_comp spec A) (ob ob' : A → oracle_comp spec B) (s : so.S)
+
+section default_simulate
+
+/-- TODO: expand this and use everywhere -/
+def default_simulate (so : simulation_oracle spec spec') (oa : oracle_comp spec A) :
+  oracle_comp spec' (A × so.S) := oa.simulate so so.default_state
+
+@[simp]
+lemma default_simulate_pure : default_simulate so (pure a) = pure (a, so.default_state) := rfl
+
+@[simp]
+lemma default_simulate_bind : default_simulate so (oa >>= ob) =
+  simulate so oa so.default_state >>= λ x, simulate so (ob x.1) x.2 := rfl
+
+@[simp]
+lemma default_simulate_query : default_simulate so (query i t) =
+  so.o i (t, so.default_state) := rfl
+
+@[simp]
+lemma support_default_simulate : (default_simulate so oa).support =
+  (simulate so oa so.default_state).support := rfl
+
+section eval_distribution
+
+variable [spec'.finite_range]
+
+lemma eval_distribution_default_simulate_pure :
+  ⦃default_simulate so (pure a)⦄ = pmf.pure (a, so.default_state) :=
+eval_distribution_simulate_pure so a so.default_state
+
+lemma eval_distribution_default_simulate_bind :
+  ⦃default_simulate so (oa >>= ob)⦄ =
+    ⦃simulate so oa so.default_state⦄ >>= λ x, ⦃simulate so (ob x.1) x.2⦄ :=
+eval_distribution_simulate_bind so oa ob so.default_state
+
+lemma eval_distribution_default_simulate_query :
+  ⦃default_simulate so (query i t)⦄ = ⦃so.o i (t, so.default_state)⦄ :=
+eval_distribution_simulate_query so i t so.default_state
+
+@[simp]
+lemma default_simulate_pure_equiv : default_simulate so (pure a) ≃ₚ
+  (pure (a, so.default_state) : oracle_comp spec' (A × so.S)) := rfl
+
+@[simp]
+lemma default_simulate_bind_equiv : default_simulate so (oa >>= ob) ≃ₚ
+  default_simulate so oa >>= λ x, simulate so (ob x.1) x.2 := rfl
+
+@[simp]
+lemma default_simulate_query_equiv : default_simulate so (query i t) ≃ₚ
+  so.o i (t, so.default_state) := rfl
+
+end eval_distribution
+
+end default_simulate
+
+section default_simulate'
+
+def default_simulate' (so : simulation_oracle spec spec') (oa : oracle_comp spec A) :
+  oracle_comp spec' A := oa.simulate' so so.default_state
+
+@[simp]
+lemma default_simulate'_pure : default_simulate' so (pure a) =
+  prod.fst <$> pure (a, so.default_state) := rfl
+
+@[simp]
+lemma default_simulate'_bind : default_simulate' so (oa >>= ob) =
+  prod.fst <$> ((simulate so oa so.default_state) >>= (λ x, simulate so (ob x.1) x.2)) := rfl
+
+@[simp]
+lemma default_simulate'_query : default_simulate' so (query i t) =
+  prod.fst <$>so.o i (t, so.default_state) := rfl
+
+@[simp]
+lemma support_default_simulate' : (default_simulate' so oa).support =
+  (simulate' so oa so.default_state).support := rfl
+
+section eval_distribution
+
+variable [spec'.finite_range]
+
+lemma eval_distribution_default_simulate'_pure : ⦃default_simulate' so (pure a)⦄ =
+  pmf.pure a := eval_distribution_simulate'_pure so a so.default_state
+
+lemma eval_distribution_default_simulate'_bind : ⦃default_simulate' so (oa >>= ob)⦄ =
+  ⦃default_simulate so oa⦄ >>= λ x, ⦃simulate' so (ob x.1) x.2⦄ :=
+eval_distribution_simulate'_bind so oa ob so.default_state
+
+lemma eval_distribution_default_simulate'_query : ⦃default_simulate' so (query i t)⦄ =
+  prod.fst <$> ⦃simulate so (query i t) so.default_state⦄ :=
+eval_distribution_simulate'_query so i t so.default_state
+
+@[simp]
+lemma default_simulate'_pure_equiv : default_simulate' so (pure a) ≃ₚ
+  (pure a : oracle_comp spec' A) :=
+simulate'_pure_equiv so a so.default_state
+
+@[simp]
+lemma default_simulate'_bind_equiv : default_simulate' so (oa >>= ob) ≃ₚ
+  (default_simulate so oa) >>= λ x, simulate' so (ob x.1) x.2 :=
+simulate'_bind_equiv so oa ob so.default_state
+
+@[simp]
+lemma default_simulate'_query_equiv : default_simulate' so (query i t) ≃ₚ
+  prod.fst <$> (so.o i (t, so.default_state)) :=
+simulate'_query_equiv so i t so.default_state
+
+end eval_distribution
+
+end default_simulate'
+
+end oracle_comp
